experiments with decidable relational graphs (failed) and start of IG (non-basic)

project/algebraic/algebraic_graph.v
@@ -1,3 +1,16 @@
+Require Import List.
+Import ListNotations.
+Require Import Bool.
+Require Import Nat.
+
+Require Import Coq.Arith.PeanoNat.
+
+Require Import Coq.Lists.ListSet.
+Require Import Coq.Arith.EqNat.
+
+Require Import Coq.Arith.Peano_dec.
+Definition eq_nat := eq_nat_dec.
+
 (* Defining an algebraic graph *)
 
 Inductive AG (A : Type) : Type :=
@@ -18,7 +31,244 @@ Coercion from_nat : nat >-> AG.
 
 
 (* *** has more priority than +++ *)
-Notation "g1 +++ g2" := (Overlay g1 g2) (at level 60, right associativity).
-Notation "g1 *** g2" := (Connect g1 g2) (at level 59, right associativity).
+Notation "ag1 +++ ag2" := (Overlay ag1 ag2) (at level 60, right associativity).
+Notation "ag1 *** ag2" := (Connect ag1 ag2) (at level 59, right associativity).
 
-(* More interesting functions will hopefully follow *)
+
+
+(* The first part of this file is just the code from the paper copied to coq,
+later on (around l.200) it becomes more experimental *)
+
+
+
+Definition edge {A : Type} (a1 a2 : A) : AG A :=
+    Connect (Vertex a1) (Vertex a2).
+
+Definition vertices {A : Type} (l : list A) : AG A :=
+    fold_right Overlay Empty (map Vertex l).
+
+Definition edges {A : Type} (l : list (A * A)) : AG A :=
+    fold_right Overlay Empty (map (fun x => edge (fst x) (snd x)) l).
+
+Definition clique {A : Type} (l : list A) : AG A :=
+    fold_right Connect Empty (map Vertex l).
+
+Compute clique [1; 2; 3; 4].
+
+Definition makeGraph {A : Type} (vs : list A) (es : list (A * A)) : AG A :=
+    Overlay (vertices vs) (edges es).
+
+
+
+Check makeGraph [1; 2; 3] [(1, 2); (2, 3)].
+Check 1 *** (2 +++ 3).
+Compute 1 *** (2 +++ 3) +++ 2 *** 3 = clique[1; 2; 3].
+
+
+Definition path {A : Type} (l : list A) : AG A :=
+    match l with
+    | [] => Empty
+    | [x] => Vertex x
+    | _::xs => edges (combine l xs)
+    end.
+
+Compute path [1; 2; 3; 4].
+
+
+Definition circuit {A : Type} (l : list A) : AG A :=
+    match l with
+    | [] => Empty
+    | x::_ => path (l ++ [x])
+    end.
+
+Compute circuit [1; 2; 3; 4].
+  
+Definition star {A : Type} (x : A) (l : list A) : AG A :=
+    Connect (Vertex x) (vertices l).
+
+Compute star 1 [2; 3; 4].
+
+
+Fixpoint gmap {A A' : Type} (f : A -> A') (ag : AG A) : AG A' := 
+    match ag with
+    | Empty => Empty
+    | Vertex x => Vertex (f x)
+    | Overlay ag1 ag2 => Overlay (gmap f ag1) (gmap f ag2)
+    | Connect ag1 ag2 => Connect (gmap f ag1) (gmap f ag2)
+    end.
+
+Compute gmap (fun x => x + 1) (1 *** 2 +++ 3 *** 4).
+
+Definition mergeVertices {A : Type} (f : A -> bool) (v : A) (ag : AG A) : AG A :=
+    gmap (fun x => if f x then v else x) ag.
+
+Fixpoint toList {A : Type} (ag : AG A) : list A :=
+    match ag with
+    | Empty => []
+    | Vertex x => [x]
+    | Overlay ag1 ag2 => toList ag1 ++ toList ag2
+    | Connect ag1 ag2 => toList ag1 ++ toList ag2
+    end.
+
+Compute toList (1 *** 2 +++ 3 *** 4).
+
+
+Fixpoint gmapVertex {A A' : Type} (f : AG A -> AG A') (ag : AG A) : AG A' :=
+    match ag with
+    | Empty => Empty
+    | Vertex x => f (Vertex x)
+    | Overlay ag1 ag2 => Overlay (gmapVertex f ag1) (gmapVertex f ag2)
+    | Connect ag1 ag2 => Connect (gmapVertex f ag1) (gmapVertex f ag2)
+    end.
+
+Definition induce {A : Type} (f : A -> bool) (ag : AG A) : AG A :=
+    gmapVertex (fun g' => match g' with
+                          | Vertex x => if f x then Vertex x else Empty
+                          | _ => g'
+                          end) ag.
+
+
+Compute induce (fun x => eqb  x  1) (1 *** 2 +++ 3 *** 4 +++ 1 *** 2).
+
+Definition removeVertex (x : nat) (ag : AG nat) : AG nat :=
+    induce (fun y => negb (eqb x y)) ag.
+
+Compute removeVertex 1 (1 *** 2 +++ 3 *** 4 +++ 1 *** 2).
+
+Definition splitVertex {A : Type} (x : nat) (l : list nat) (ag : AG nat) : AG nat :=
+    gmapVertex (fun g' => match g' with
+                          | Vertex y => if eqb x y then vertices l else Vertex y
+                          | _ => g'
+                          end) ag.
+
+Compute splitVertex 1 [0; 1] (1 *** (2 +++ 3)).
+
+Fixpoint removeEdge (x y : nat) (ag : AG nat) : AG nat :=
+    match ag with
+    | Empty => Empty
+    | Vertex z => Vertex z
+    | Overlay ag1 ag2 => Overlay (removeEdge x y ag1) (removeEdge x y ag2)
+    | Connect ag1 ag2 => Overlay (Connect (removeVertex x ag1) ag2) (Connect ag1 (removeVertex y ag2))
+    end.
+    
+    
+  
+Compute removeEdge 1 2 (1 *** 2 +++ 3 *** 4).
+
+
+
+Fixpoint transpose {A : Type} (ag : AG A) : AG A :=
+    match ag with
+    | Empty => Empty
+    | Vertex x => Vertex x
+    | Overlay ag1 ag2 => Overlay (transpose ag1) (transpose ag2)
+    | Connect ag1 ag2 => Connect (transpose ag2) (transpose ag1)
+    end.
+
+
+
+
+
+
+
+
+
+
+
+
+
+
+
+
+
+(* Here, I start deviating from the paper: *)
+
+
+
+(* These functions assume no overlapping node labels. It thinks that 1 *** 1 has 2 nodes *)
+
+
+Fixpoint AG_toList {A : Type} (ag : AG A) : list A :=
+    match ag with
+    | Empty => []
+    | Vertex x => [x]
+    | Overlay ag1 ag2 => AG_toList ag1 ++ AG_toList ag2
+    | Connect ag1 ag2 => AG_toList ag1 ++ AG_toList ag2
+    end.
+
+
+Compute AG_toList (1 *** 2 +++ 3 *** 4).
+Compute AG_toList (1 *** 2 +++ 1 *** 2).
+Compute AG_toList (1 *** 1).
+Compute AG_toList (1 +++ 1).
+
+
+
+Fixpoint countNodes {A : Type} (ag : AG A) : nat :=
+    match ag with
+    | Empty => 0
+    | Vertex x => 1
+    | Overlay ag1 ag2 => countNodes ag1 + countNodes ag2
+    | Connect ag1 ag2 => countNodes ag1 + countNodes ag2
+    end.
+
+Fixpoint countEdges {A : Type} (ag : AG A) : nat :=
+    match ag with
+    | Empty => 0
+    | Vertex x => 0
+    | Overlay ag1 ag2 => countEdges ag1 + countEdges ag2
+    | Connect ag1 ag2 => countEdges ag1 + countEdges ag2 + countNodes ag1 * countNodes ag2
+    end.
+
+
+Compute countNodes (1 *** 2 +++ 3 *** 4).
+Compute countNodes (1 *** 2 +++ 1 *** 2).
+
+
+
+
+
+(* This a somewhat analogous to DFS *)
+(* A little magical, since we are using the returned list as a output list as well as a set *)
+Fixpoint searchGraphUnique (ag : AG nat) (s : set nat) : (list nat) :=
+    match ag with
+    | Empty => []
+    | Vertex x => if set_mem eq_nat x s then [] else [x]
+    | Overlay ag1 ag2 => match searchGraphUnique ag1 s with
+                        | ret => ret ++ searchGraphUnique ag2 (set_union eq_nat s ret)
+                        end
+    | Connect ag1 ag2 => match searchGraphUnique ag1 s with
+                        | ret => ret ++ searchGraphUnique ag2 (set_union eq_nat s ret)
+                        end
+    end.
+
+(* This is somewhat analogous, but for BFS, but Coq needs more evidence of decreasing argument,
+it would need a queue data structure and *)
+(* Fixpoint searchGraphUnique' (target : nat) (g : graph nat) : bool :=
+  let fix bfs_queue (queue : list (graph nat)) (visited : list nat) : bool :=
+    match queue with
+    | [] => false
+    | Empty :: rest => bfs_queue rest visited
+    | Vertex x :: rest =>
+        if (x =? target) then true
+        else bfs_queue rest (visited ++ [x])
+    | Overlay top bottom :: rest => 
+        let new_queue := rest ++ [top] ++ [bottom] in
+        bfs_queue new_queue visited
+    | Connect gleft gright :: rest => 
+        let new_queue := rest ++ [gleft] ++ [gright] in
+        bfs_queue new_queue visited
+    end
+  in
+  bfs_queue [g] []. *)
+
+
+
+Compute searchGraphUnique (1 *** 2 +++ 3 *** 4) [].
+Compute searchGraphUnique (1 *** 2 +++ 1 *** 2) [].
+Compute searchGraphUnique (1 *** 1) [].
+Compute searchGraphUnique (1 +++ 1) [].
+
+Compute searchGraphUnique (1 *** 2 +++ 2 *** 3 +++ 1 *** 3) [].
+
+
