project/inductive/inductive_graph.v
@@ -6,313 +6,137 @@ Require Import Bool.
 Require Import List.
 Import ListNotations.
 
+Require Import MyProject.project.util.NatMap.
+Require Import MyProject.project.util.NatSet.
+Open Scope nat_scope.
+
 (* This file defines an inductive graph using maps like Erwig *)
 (* Note that A is the node label type and B is the edge label type *)
 (* At the moment, there are only the "MINIMAL" implementations  *)
-(* TODO: full IG are currently in an incomplete state... *)
 
-(*
-(* info: for verification, I either write algebraic specifications using these (no need for "well-formedness"),
-or I "implement" all of them an show that they are correct for relational graphs and then show _isomorphism_ (here, yes need for "well-formedness")
-  for the translation to relational graphs, I would formally need to show "complete" and "correctness" (like they do for elements in BST)
-  I would also need to implement "at least some of these operations" for relational graphs *)
-class Graph gr where
-  {-# MINIMAL empty, isEmpty, match, mkGraph, labNodes #-}
-
-  -- | An empty 'Graph'.
-  empty     :: gr a b
-
-  -- | True if the given 'Graph' is empty.
-  isEmpty   :: gr a b -> Bool
-
-  -- | Decompose a 'Graph' into the 'MContext' found for the given node and the
-  -- remaining 'Graph'.
-  match     :: node -> gr a b -> Decomp gr a b
-
-  -- | Create a 'Graph' from the list of 'LNode's and 'LEdge's.
-  --
-  --   For graphs that are also instances of 'DynGraph', @mkGraph ns
-  --   es@ should be equivalent to @('insEdges' es . 'insNodes' ns)
-  --   'empty'@.
-  mkGraph   :: [LNode a] -> [LEdge b] -> gr a b
-
-  -- | A list of all 'LNode's in the 'Graph'.
-  labNodes  :: gr a b -> [LNode a]
-
-  -- | Decompose a graph into the 'Context' for an arbitrarily-chosen 'Node'
-  -- and the remaining 'Graph'.
-  matchAny  :: gr a b -> GDecomp gr a b
-
-  -- | The number of 'Node's in a 'Graph'.
-  noNodes   :: gr a b -> Int
-
-  -- | The minimum and maximum 'Node' in a 'Graph'.
-  nodeRange :: gr a b -> (Node,Node)
-
-  -- | A list of all 'LEdge's in the 'Graph'.
-  labEdges  :: gr a b -> [LEdge b]
+(*{-# MINIMAL empty, isEmpty, match, mkGraph, labNodes #-}
   *)
 
-
-(* https://rocq-prover.org/doc/v8.9/stdlib/Coq.FSets.FMapList.html *)
-Require Import Coq.FSets.FMapInterface.
-Require Import Coq.FSets.FMapList.
-(* Require Import Coq.FSets.FMapAVL. *)
-Require Import Coq.FSets.FMapFacts.
-Require Import Coq.Structures.OrderedTypeEx.
-
-Definition node := Nat_as_OT.t.
-
-Module NatMap := FMapList.Make(Nat_as_OT).
-(* Module NatMap := FMapAVL.Make(Nat_as_OT). *)
-
-
-Open Scope nat_scope.
-
-(* In case, I want to go polymorphic some day *)
-(* Definition Adj (A : Type) := list (A * node).
+Definition Adj (B : Type) := list (B * Node). 
 
 Definition Context (A B : Type) : Type :=
-    (Adj B * node * A * Adj B).
+    (Adj B * Node * A * Adj B).
 
 Definition MContext (A B : Type) : Type :=
     option (Context A B).
 
-Definition Decomp (Graph : Type -> Type -> Type) (A B : Type) : Type :=
-  (MContext A B * Graph A B). *)
 
-
-(* Todo: this is incorrect, since according to the paper, multigraphs are allowed, which this does not permit *)
-(* This should be some "multimap" *)
-Definition Adj' (B : Type) := NatMap.t B.
+(* Definition Adj' (B : Type) := NatMap.t (list B). *)
 
 (* No node needed, since the node is the key *)
 Definition Context' (A B : Type) : Type :=
-  (Adj' B * A * Adj' B).
+  (Adj B * A * Adj B).  
+
+Definition IG (A B : Type) := NatMap.t (Context' A B).
+
+Definition Decomp (A B : Type) : Type :=
+  (MContext A B * IG A B). 
 
 
-Definition MContext' (A B : Type) : Type :=
-    option (Context' A B).
-
-
-
-Definition bind {A B : Type} (ig : option A) (f : A -> option B) : option B :=
-  match ig with
-  | None => None
-  | Some a => f a
-  end.
-
-
-Require Import Coq.FSets.FSetList.
-Require Import Coq.FSets.FSetEqProperties.
-
-Module NatSet := FSetList.Make(Nat_as_OT).
-Print FSetEqProperties.
-Module NatSetProperties := FSetEqProperties.EqProperties(NatSet).
-
-
-
-
-(* Returns None, if there are duplicates *)
-Definition set_from_list (l : list node) : option NatSet.t :=
-  fold_right (fun (k : node) (acc : option NatSet.t) =>
-                bind acc (fun (acc : NatSet.t) => if NatSet.mem k acc then None else Some (NatSet.add k acc))
-              ) (Some NatSet.empty) l.
-
-  
-
-Definition IG_map_out_keys {A B : Type} (IG_data : NatMap.t (Context' A B)) : option NatSet.t :=
-  set_from_list (
-    concat (
-      map (fun '((_, (_, _, out_map)) : (node * Context' A B)) => map fst (NatMap.elements out_map))
-        
-      (NatMap.elements IG_data)
-    )
-  )
-.
-
-
-Definition IG_map_in_keys {A B : Type} (IG_data : NatMap.t (Context' A B)) : option NatSet.t :=
-  set_from_list (
-    concat (
-      map ( fun '((_, (in_map, _, t_step)) : (node * Context' A B)) => map fst (NatMap.elements in_map))
-      (NatMap.elements IG_data)
-    )
-  )
-.
-
-Definition IG_nodes_keys {A B : Type} (IG_data : NatMap.t (Context' A B)) : option NatSet.t :=
-  set_from_list (map fst (NatMap.elements IG_data))
-.
-
-
-Definition IG_valid_cond_fun {A B : Type} (IG_data : NatMap.t (Context' A B)) : bool :=
-  let in_keys := IG_map_in_keys IG_data in
-  let out_keys := IG_map_out_keys IG_data in
-
-  let edge_diffs := bind in_keys (fun (in_keys : NatSet.t) => bind out_keys
-                                  (fun (out_keys : NatSet.t) => Some (NatSet.diff in_keys out_keys))) in
-
-  let edge_keys := bind in_keys (fun (in_keys : NatSet.t) => bind out_keys
-                                  (fun (out_keys : NatSet.t) => Some (NatSet.union in_keys out_keys))) in
-
-  
-  let node_keys := IG_nodes_keys IG_data in
-
-  match edge_diffs, edge_keys, node_keys with
-  | Some edge_diffs, Some edge_keys, Some node_keys =>
-    NatSet.is_empty edge_diffs && NatSet.equal edge_keys node_keys
-  | _, _, _ => false
-  end
-.
-  
-
-Definition _valid_cond {A B : Type} (IG_data : NatMap.t (Context' A B)) : Prop :=
-  IG_valid_cond_fun IG_data = true.
-
-
-
-Definition IG_data_unsafe (A B : Type) : Type :=
-  NatMap.t (Context' A B).
-  
-(* Map instead of list *)
-Record IG (A B : Type) := {
-  IG_data : IG_data_unsafe A B;
-  IG_valid : _valid_cond IG_data
-}.
-
-Arguments IG_data {A B}.
-Arguments IG_valid {A B}.
-
-(* These are shared with RG_valid_prover *)
-Ltac IG_valid_prover := unfold _valid_cond; firstorder.
-(* Ltac IG_valid_prover_with rg := pose proof rg.(RG_valid); unfold valid_cond; firstorder.
-Ltac IG_valid_prover_withs rg1 rg2 := pose proof rg1.(RG_valid); pose proof rg2.(RG_valid); unfold valid_cond; firstorder. *)
-
-
-Definition Decomp' (A B : Type) : Type :=
-  (MContext' A B * IG A B).
-
-Definition LNode (A : Type) : Type := (node * A).
-Definition LEdge (B : Type) : Type := (node * node * B).
-
-
-
-
-
-
-
-
+Definition LNode (A : Type) : Type := (Node * A).
+Definition LEdge (B : Type) : Type := (Node * Node * B).
 
 
 
 
 
 (* Start defining functionality: *)
-Definition empty {A B : Type} : IG A B.
-Proof.
-  refine ({|
-    IG_data := NatMap.empty (Context' A B);
-    IG_valid := _
-  |}).
-  IG_valid_prover.
-Defined.
+Definition IG_empty {A B : Type} : IG A B :=
+  NatMap.empty (Context' A B).
+
+
+Definition IG_isEmpty {A B : Type} (ig : IG A B) : bool :=
+  NatMap.is_empty ig.
+
+Compute IG_isEmpty IG_empty.
 
 
 
-Definition isEmpty {A B : Type} (ig : IG A B) : bool :=
-  NatMap.is_empty ig.(IG_data).
-
-Compute isEmpty empty.
+(* Here start the helper functions for "match" *)
 
 
-(* Here start the helper functions for "matsh". match is a reserved keyword by coq.... *)
+
 
 (* Applies a function to a map entry if it exists quickly *)
-Definition update_entry {A B : Type} (n : node) (f : Context' A B -> Context' A B) (ig : IG_data_unsafe A B) : IG_data_unsafe A B :=
-  match NatMap.find n ig with
-    | Some v => NatMap.add n (f v) ig
+Definition _updateEntry {A B : Type} (node : Node) (f : Context' A B -> Context' A B) (ig : IG A B) : IG A B := 
+  match NatMap.find node ig with
+    | Some v => NatMap.add node (f v) ig
     | None => ig
   end.
 
-
-
-Definition clean_up_helper {A B : Type} (n : node) (outs_with_n ins_with_n : list node) (ig : IG_data_unsafe A B) : IG_data_unsafe A B :=
-  (* Loop over ingoing edges of removed node to update the outgoing of all of those to not have n anymore *)
-  let x' := fold_right (fun (elem : node) (acc : IG_data_unsafe A B) =>
-    update_entry elem (fun '(in_map', key', out_map') => (in_map', key', NatMap.remove n out_map'))
-    acc) ig outs_with_n in
-  (* Loop over outgoing edges of removed node to update the ingoing of all of those to not have n anymore *)
-  fold_right (fun (elem : node) (acc : IG_data_unsafe A B) =>
-    update_entry elem (fun '(in_map', key', out_map') =>  (NatMap.remove n in_map', key', out_map'))
-    acc) x' ins_with_n
-.
-
-
-Definition clean_up {A B : Type} (n : node) (context : Context' A B) (ig : IG_data_unsafe A B) : IG_data_unsafe A B :=
-  match context with
-    | (in_map, _, out_map) =>
+Definition _addSucc {A B : Type} (node : Node) (label : B) (context' : Context' A B) : Context' A B :=
+  match context' with
+  | (froms, l, tos) => (froms, l, (label, node) :: tos)
+  end.
   
-      let outs_with_n := map fst (NatMap.elements in_map) in
-      let ins_with_n := map fst (NatMap.elements out_map) in
-      clean_up_helper n outs_with_n ins_with_n (NatMap.remove n ig)
-  
+Definition _addPred {A B : Type} (node : Node) (label : B) (context' : Context' A B) : Context' A B :=
+  match context' with
+  | (froms, l, tos) => ((label, node) :: froms, l, tos)
   end.
 
 
-
-Definition matsh {A B : Type} (n : node) (ig : IG A B) : Decomp' A B.
-Proof.
-  pose
-  match NatMap.find n ig.(IG_data) with
-  | None => (None, empty.(IG_data))
-  | Some context as mContext => (mContext, clean_up n context ig.(IG_data)) 
-  end as intermediate_computation.
-  split.
-  - destruct intermediate_computation as [mContext x']. apply mContext.
-  - destruct intermediate_computation as [mContext x'].
-  refine ({|
-    IG_data := x';
-    IG_valid := _
-  |}).
-  IG_valid_prover.
-
-Admitted.
+Definition _clearSucc {A B : Type} (node : Node) (context' : Context' A B) : Context' A B :=
+  match context' with
+  | (froms, label, tos) => (froms, label, filter (fun '(_, n) => negb (n =? node)) tos)
+  end.
 
 
+Definition _clearPred {A B : Type} (node : Node) (context' : Context' A B) : Context' A B :=
+  match context' with
+  | (froms, label, tos) => (filter (fun '(_, n) => negb (n =? node)) froms, label, tos)
+  end.
 
 
+Definition _updAdj {A B : Type} (adj : Adj B) (f : B -> Context' A B -> Context' A B) (gr : IG A B) : IG A B :=
+  fold_right (fun '(l, n) (acc : IG A B) => _updateEntry n (f l) acc) gr adj.  
+
+
+Definition _cleanSplit {A B : Type} (node : Node) (context' : Context' A B) (ig : IG A B) : Context A B * IG A B :=
+  match context' with
+  | (froms, label, tos) =>
+                          let rmLoops :=  filter (fun '(_, n) => negb (n =? node)) in
+                          let froms' := rmLoops froms in
+                          let tos' := rmLoops tos in
+                          let context := (froms', node, label, tos (*no '*)) in
+                          
+                          let ig' := _updAdj froms' (fun x y => _clearPred node y) ig in
+                          let ig'' := _updAdj tos' (fun x y => _clearSucc node y) ig' in
+                          (context, ig'')
+  end.
+
+
+Definition IG_match {A B : Type} (node : Node) (ig : IG A B) : Decomp A B :=
+  match NatMap.find node ig with
+  | None => (None, ig)
+  | Some context' => match _cleanSplit node context' (NatMap.remove node ig) with
+                    | (context, ig') => (Some context, ig')
+                    end
+  end.
 
 
 
 
 (* Here start the helper functions for "mkGraph" *)
 
-
 (* This is the "&" constructor, but it has to be defined as a function, since it is too advanced *)
-Definition add {A B : Type} (n : node) (node : Context' A B) (ig : IG A B) : IG A B.
-Proof.
-  refine ({|
-    IG_data := NatMap.add n node ig.(IG_data);
-    IG_valid := _
-  |}).
-  IG_valid_prover.
-Admitted.
+Definition add {A B : Type} (context : Context A B) (ig : IG A B) : IG A B :=
+  match context with
+  | (froms, node, label, tos) =>
+                                let ig' := NatMap.add node (froms, label, tos) ig in
+                                let ig'' := _updAdj tos (_addPred node) ig' in
+                                _updAdj froms (_addSucc node) ig''
+  end.
 
 
-
-
-Definition insNode {A B : Type} (node : LNode A) (ig : IG A B) : IG A B.
-Proof.
-  refine ({|
-    IG_data :=   match node with
-    | (v, l) => (add v (NatMap.empty B, l, NatMap.empty B) ig).(IG_data)
-    end;
-    IG_valid := _
-  |}).
-Admitted.
-
-
+Definition insNode {A B : Type} (node : LNode A) (ig : IG A B) : IG A B :=
+  match node with
+  | (n, l) => add ([], n, l, []) ig
+  end.
 
 Definition insNodes {A B : Type} (nodes : list (LNode A)) (ig : IG A B) : IG A B :=
   fold_right insNode ig nodes.
@@ -321,35 +145,27 @@ Definition insNodes {A B : Type} (nodes : list (LNode A)) (ig : IG A B) : IG A B
 
 
 
-Definition insEdge {A B : Type} (edge : LEdge B) (ig : IG A B) : IG A B.
-Proof.
-  refine ({|
-    IG_data := match edge with
-    | (v,w,l) =>  update_entry v (fun '(in_map, key', out_map) => (in_map, key', NatMap.add w l out_map))
-                  (
-                  (* Now update the other side of the edge *)
-                  update_entry w (fun '(in_map, key', out_map) => (NatMap.add v l in_map, key', out_map))
-                  ig.(IG_data)
-                  )
-    end;
-    IG_valid := _
-  |}).
-Admitted.
-
-
-
+Definition insEdge {A B : Type} (edge : LEdge B) (ig : IG A B) : IG A B :=
+  match edge with
+  | (from, to, l) =>
+                    let (mcxt, ig') := IG_match from ig in
+                    match mcxt with
+                    | (Some (froms, _, label, tos)) => add (froms, from, label, (l, to) :: tos) ig'
+                    | None => ig
+                    end
+  end.
+                    
 Definition insEdges {A B : Type} (edges : list (LEdge B)) (ig : IG A B) : IG A B :=
   fold_right insEdge ig edges.
 
 
 
 Definition mkGraph {A B : Type} (nodes : list (LNode A)) (edges : list (LEdge B)) : IG A B :=
-  insEdges edges (insNodes nodes empty).
-
+  insEdges edges (insNodes nodes IG_empty).
 
  
 Definition labNodes {A B : Type} (ig : IG A B) : list (LNode A) :=
-  map (fun '(v, (_, l, _)) => (v,l)) (NatMap.elements ig.(IG_data)).
+  map (fun '(v, (_, l, _)) => (v,l)) (NatMap.elements ig).
 
 
 
@@ -360,39 +176,11 @@ Definition labNodes {A B : Type} (ig : IG A B) : list (LNode A) :=
 
 (* Make IGs visible  *)
 
-
-
 Definition show_IG {A B : Type} (ig : IG A B) :=
-  map (fun '(k, (in_m, lab, out_m)) => (k, (NatMap.elements in_m, lab, NatMap.elements out_m))) (NatMap.elements ig.(IG_data)).
+  NatMap.elements ig. 
 
-Definition show_Context {A B : Type} (con : Context' A B) :=
-  match con with
-  | (in_map, key, out_map) => (NatMap.elements in_map, key, NatMap.elements out_map)
-  end.
-
-
-Definition show_MContext {A B : Type} (mContext : MContext' A B) :=
-  option_map (fun con => show_Context con) mContext.
-
-
-Definition show_MContext_lame {A B : Type} (mContext : MContext' A B) :=
-  match mContext with
-  | None => None
-  | Some con => Some (show_Context con)
-  end.
-
-
-Definition show_Decomp {A B : Type} (d : Decomp' A B) :=
+Definition show_Decomp {A B : Type} (d : Decomp A B) :=
   match d with
-  | (mContext, x) => (show_MContext mContext, show_IG x)
+  | (mContext, x) => (mContext, show_IG x)
   end
 .
-
-
-
-(* Helpers for proving correctness: *)
-Definition lookup {X Y : Type} (n : node) (ig : IG X Y) : option X :=
-  option_map (fun c => match c with (_, label, _) => label end) (NatMap.find n ig.(IG_data)).
-  
-
-
