project/algebraic/algebraic_graph_simplification.v
@@ -1,0 +1,103 @@
+Require Import MyProject.project.algebraic.algebraic_graph.
+
+
+(* Associate *** *)
+Fixpoint Setp_O {A : Type} (ag : AG A) : AG A :=
+  match ag with
+  | Empty => Empty
+  | Vertex x => Vertex x
+  | (ag1 *** ag2) *** ag3 => Setp_O ag1 *** (Setp_O ag2 *** Setp_O ag3)
+  | ag1 +++ ag2 => Setp_O ag1 +++ Setp_O ag2
+  | ag1 *** ag2 => Setp_O ag1 *** Setp_O ag2
+  end.
+
+(* Distribute *** over +++ *)
+Fixpoint Setp_1 {A : Type} (ag : AG A) : AG A :=
+  match ag with
+  | Empty => Empty
+  | Vertex x => Vertex x
+  | ag1 *** (ag2 +++ ag3) => (Setp_1 ag1 *** Setp_1 ag2) +++ (Setp_1 ag1 *** Setp_1 ag3)
+  | (ag1 +++ ag2) *** ag3 => (Setp_1 ag1 *** Setp_1 ag3) +++ (Setp_1 ag2 *** Setp_1 ag3)
+  | ag1 +++ ag2 => Setp_1 ag1 +++ Setp_1 ag2
+  | ag1 *** ag2 => Setp_1 ag1 *** Setp_1 ag2
+  end.
+
+
+(* Decompose *** *** *)
+Fixpoint Setp_2 {A : Type} (ag : AG A) : AG A :=
+  match ag with
+  | Empty => Empty
+  | Vertex x => Vertex x
+  | ag1 *** (ag2 *** ag3) => Setp_2 ag1 *** Setp_2 ag2 +++ (Setp_2 ag1 *** Setp_2 ag3 +++ Setp_2 ag2 *** Setp_2 ag3)
+  | ag1 +++ ag2 => Setp_2 ag1 +++ Setp_2 ag2
+  | ag1 *** ag2 => Setp_2 ag1 *** Setp_2 ag2
+  end.
+
+
+
+
+(* Associate +++ *)
+Fixpoint Setp_3 {A : Type} (ag : AG A) : AG A :=
+  match ag with
+  | Empty => Empty
+  | Vertex x => Vertex x
+  (* Here, Setp_3 should probably be called on the whole expression once more (in similar other places probably too), but fixpoint does not allow it *)
+  | (ag1 +++ ag2) +++ ag3 => Setp_3 ag1 +++ (Setp_3 ag2 +++ Setp_3 ag3)
+  | ag1 +++ ag2 => Setp_3 ag1 +++ Setp_3 ag2
+  | ag1 *** ag2 => Setp_3 ag1 *** Setp_3 ag2
+  end.
+
+Definition All_Setp {A : Type} (ag : AG A) : AG A :=
+    Setp_3
+     (Setp_2 (Setp_1
+    (Setp_O ag)
+    )
+    )
+.
+
+Compute All_Setp (1 *** 2 +++ 3 *** 4).
+Compute All_Setp (1 *** (2 *** 3)).
+(* big, compilicated example *)
+Compute All_Setp (1 *** (2 +++ 3) +++ 4 *** (5 +++ (6 *** 7)) +++ 8).
+(* here, the simplification breaks *)
+Compute All_Setp (1 *** 2 +++ ((4 *** 6 *** 7)) +++ 8). 
+
+Compute All_Setp (((((2 +++ 4) +++ 6) +++ 3))).
+Compute All_Setp (1 +++ 2 +++ 3 +++ 4).
+
+
+
+
+(* Conversion to relational representation, for euality checking: *)
+
+(* Fixpoint toSet' (ag : AG nat) : fSetAVLNatGraph :=
+    match g with
+    | Empty => empty_graphAVL
+    | Vertex x => insNodeAVL empty_graphAVL x
+    | Overlay ag1 ag2 => unionGraphsAVL (toSet' g1) (toSet' g2)
+    | Connect ag1 ag2 =>
+        match (toSet' g1, toSet' g2) with
+        | ((from_nodes, from_edges) as g1', (to_nodes, to_edges) as g2')
+            => insEdgesAVL (unionGraphsAVL g1' g2') (setProdAVL from_nodes to_nodes)
+        end
+    end.
+
+Check fold_right.
+
+Definition fromSet' (g : fSetAVLNatGraph) : graph nat :=
+    match g with
+    | (nodes, edges) => fold_right Overlay Empty (map (fun x => Vertex x) (NS.elements nodes)) +++ 
+                        fold_right Overlay Empty (map (fun x => Connect (Vertex (fst x)) (Vertex (snd x))) (PS.elements edges))
+    end.
+
+
+
+Definition buildCanonicalForm'' (ag :graph nat) : graph nat :=
+    fromSet (toSet g).
+
+
+
+Compute buildCanonicalForm'' (1 *** 2 +++ 3 *** 4).
+Compute buildCanonicalForm'' (1 *** (2 +++ 3)).
+
+Compute elementsAVL (toSet' (1 *** 2 +++ 3 *** 4)). *)
