project/relational_graph_IG_operations_advanced.v
@@ -1,0 +1,285 @@
+Require Import String.
+Open Scope string_scope.
+
+Require Import List.
+Import ListNotations.
+
+(*
+Require Import Coq.Arith.Arith.
+
+Require Import Bool.
+
+
+Require Import MyProject.project.util.util.
+
+Require Import MyProject.project.relational_graph_theory.
+
+
+Require Import Coq.Sets.Ensembles.
+Require Import MyProject.project.util.NatSet.
+*)
+
+Require Import Coq.Relations.Relation_Definitions.
+Require Import Coq.Relations.Relation_Operators.
+Require Import Coq.Sets.Ensembles.
+
+Require Import MyProject.project.util.util.
+Require Import MyProject.project.relational_graph.
+Require Import MyProject.project.relational_graph_IG_operations.
+
+
+(* Auxiliary graph class functions: *)
+Definition RG_matchAny {A B : Type} (rg : RG A B) : RG_Decomp A B.
+Proof. Admitted.
+   (* :=
+  let isValid := exists node, rg.(RG_nodes) node in
+  (isValid, ((fun l (from : A) => isValid /\ rg.(RG_edges) from node l),
+              node,
+              (fun l (to : A) => isValid /\ rg.(RG_edges) node to l)))
+. *)
+
+(* Difficult, as lack of decidability *)
+Definition RG_noNodes {A B : Type} (rg : RG A B) : nat.
+Proof. Admitted.
+  
+(* RG_nodeRange makes no sense, as As are not ordered *)
+  (* Definition RG_nodeRange {A B : Type} (rg : RG A B) : (A, A). *)
+
+
+Definition RG_labEdges {A B : Type} (rg : RG A B) : _edgeRelation A B :=
+  rg.(RG_edges).
+
+
+Require Import Recdef. (* Must import this to use the Function feature *)
+
+(* This is a problem *)
+Definition RG_measure {A B : Type} (rg : RG A B) : nat.
+Proof. Admitted.
+
+Function RG_gmap {A B C D : Type} (f : RG_Context A B -> RG_Context C D) (rg : RG A B) {measure RG_measure rg} : RG C D :=
+  match RG_matchAny rg with
+    | ((True, c), rest) => _add (f c) (RG_gmap f rest)
+    (* | ((False, c), rest) => _add (f c) (RG_gmap f rest) *)
+  end
+.
+Proof. Admitted.
+
+
+
+Definition RG_grev {A B : Type} (rg : RG A B) : RG A B :=
+  RG_gmap _ _ _ _ (fun '((froms, node, tos) : RG_Context A B) => (tos, node, froms)) rg
+.
+
+Function RG_ufold {A B C : Type} (f : RG_Context A B -> C -> C) (acc : C) (rg : RG A B) {measure RG_measure rg} : C :=
+  match RG_matchAny rg with
+    | ((True, c), rest) => f c (RG_ufold f acc rest)
+    (* | ((False, c), rest) => _add (f c) (RG_gmap f rest) *)
+  end
+.
+Proof. Admitted.
+
+
+Definition RG_gmap' {A B C D : Type} (f : RG_Context A B -> RG_Context C D) (rg : RG A B) : RG C D :=
+  RG_ufold _ _ (RG C D) (fun (c : RG_Context A B) (acc : RG C D) => _add (f c) acc) RG_empty rg.
+
+
+Definition RG_nodes' {A B : Type} (rg : RG A B) : list A :=
+  RG_ufold _ _ _ (fun '(froms, node, tos) acc => node :: acc ) [] rg.
+  
+Definition RG_undir {A B : Type} (rg : RG A B) : RG A B :=
+  RG_gmap _ _ _ _ (fun '(froms, node, tos) =>
+    let fromsTos := (fun (b : B) (a : A) => froms b a \/ tos b a) in
+    (fromsTos, node, fromsTos)) rg
+.
+
+Definition RG_gsuc {A B : Type} (node : A) (rg : RG A B) : Ensemble A :=
+  match RG_match node rg with
+    | ((True, (_, _, tos)), rest) => fun (a : A) => exists l, tos l a 
+  end
+.
+
+(* RG_deg is hard to implement, as is is hard to count *)
+Definition RG_deg {A B : Type} (node : A) (rg : RG A B) : nat.
+Proof. Admitted.
+(* :=
+  match RG_match node rg with
+    | ((True, (froms, nodeAgain, tos)), rest) => fun (a : A) => CARDINALITY froms tos 
+  end
+. *)
+
+Definition RG_del {A B : Type} (node : A) (rg : RG A B) : RG A B :=
+  match RG_match node rg with
+    | ((True, _), rest) => rest
+  end
+.
+
+Definition RG_suc {A B : Type} (node : A) (c : RG_Context A B) : Ensemble A :=
+  match c with | (_, _, tos) =>
+    fun (a : A) => exists l, tos l a 
+  end
+.
+
+
+
+(* More advanced stuff *)
+
+dfs :: [Node] → Graph a b → [Node]
+dfs [ ]
+g
+= []
+v
+dfs (v :vs) (c & g) = v :dfs (suc c++vs) g
+dfs (v :vs) g
+= dfs vs g
+
+(* Possible extensions: *)
+dfs vs Empty = [ ]
+dfs vs g | null vs || isEmpty g = [ ]
+
+
+dfs [ ]
+g0 = [ ]
+dfs (v :vs) g 0 = case match v g 0 of
+(Just c, g) → v :dfs (suc c++vs) g
+(Nothing, g) → dfs vs g
+
+data Tree a = Br a [Tree a]
+postorder :: Tree a → [a]
+postorder (Br v ts) = concatMap postorder ts++[v ]
+
+concatMap :: (a → [b]) → [a] → [b]
+concatMap f = concat . map f
+
+
+df :: [Node] → Graph a b → ([Tree Node], Graph a b)
+df [ ]
+g
+= ([ ], g)
+v
+df (v :vs) (c & g) = (Br v f :f 0 , g2 ) where (f , g1 ) = df (suc c) g
+(f 0 , g2 ) = df vs g1
+df (v :vs) g
+= df vs g
+
+dff :: [Node] → Graph a b → [Tree Node]
+dff vs g = fst (df vs g)
+
+
+topsort :: Graph a b → [Node]
+topsort = reverse . concatMap postorder . dff
+scc :: Graph a b → [Tree Node]
+scc g = dff (topsort g) (grev g)
+
+
+
+
+(* BFS *)
+
+bfs :: [Node] → Graph a b → [Node]
+bfs [ ]
+g
+= []
+v
+bfs (v :vs) (c & g) = v :bfs (vs++suc c) g
+bfs (v :vs) g
+= bfs vs g
+
+type Path = [Node]
+type RTree = [Path]
+bft :: Node → Graph a b → RTree
+bft v = bf [[v ]]
+bf :: [Path] → Graph a b → RTree
+bf [ ]
+g
+= []
+v
+bf (p@(v : ):ps) (c & g) = p:bf (ps++map (:p) (suc c)) g
+bf (p:ps)
+g
+= bf ps g
+
+
+first :: (a → Bool ) → [a] → a
+first p = head . filter p
+esp :: Node → Node → Graph a b → Path
+esp s t = reverse . first (\(v : ) → v t) . bft s
+
+
+(* Shortest path: *)
+
+type LNode a = (Node, a)
+type LPath a = [LNode a]
+type LRTree a = [LPath a]
+instance Eq a ⇒ Eq (LPath a) where
+(( , x ): ) (( , y): ) = x y
+instance Ord a ⇒ Ord (LPath a) where
+(( , x ): ) < (( , y): ) = x < y
+getPath :: Node → LRTree a → Path
+getPath v = reverse . map fst . first (\((w , ): ) → w == v)
+
+
+
+expand :: Real b ⇒ b → LPath b → Context a b → [Heap (LPath b)]
+expand d p ( , , , s) = map (\(l , v ) → unitHeap ((v , l + d ):p)) s
+dijkstra :: Real b ⇒ Heap (LPath b) → Graph a b → LRTree b
+dijkstra h g | isEmptyHeap h || isEmpty g = [ ]
+v
+dijkstra (p@((v , d ): )≺h) (c & g) = p:dijkstra (mergeAll (h:expand d p c)) g
+dijkstra ( ≺h) g
+= dijkstra h g
+
+
+
+
+spt :: Real b ⇒ Node → Graph a b → LRTree b
+spt v = spt (unitHeap [(v , 0)])
+sp :: Real b ⇒ Node → Node → Graph a b → Path
+sp s t = getPath t . spt s
+
+
+
+(* Minimum spanning tree *)
+addEdges :: Real b ⇒ LPath b → Context a b → [Heap (LPath b)]
+addEdges p ( , , , s) = map (\(l , v ) → unitHeap ((v , l ):p)) s
+
+mst :: Real b ⇒ Node → Graph a b → LRTree b
+mst v g = prim (unitHeap [(v , 0)]) g
+prim :: Real b ⇒ Heap (LPath b) → Graph a b → LRTree b
+prim h g | isEmptyHeap h || isEmpty g = [ ]
+v
+prim (p@((v , ): )≺h) (c & g) = p:prim (mergeAll (h:addEdges p c)) g
+prim ( ≺h) g
+= prim h g
+
+mstp :: Real b ⇒ LRTree b → Node → Node → Path
+mstp t a b = joinPaths (getPath a t) (getPath b t)
+joinPaths :: Path → Path → Path
+joinPaths p q = joinAt (head p) (tail p) (tail q)
+joinAt :: Node → Path → Path → Path
+joinAt x (v :vs) (w :ws) | v w = joinAt v vs ws
+joinAt x p
+q
+= reverse p++(x :q)
+
+
+
+(* Maximum independent node set: *)
+
+
+indep :: Graph a b → [Node]
+indep Empty = [ ]
+indep g
+= if length i1 > length i2 then i1 else i2
+where vs
+= nodes g
+m
+= maximum (map (flip deg g) vs)
+v
+= first (\v → deg v g m) vs
+v
+c & g0 = g
+i1
+= indep g 0
+i2
+= v :indep (foldr del g 0 (pre c++suc c))
+
