project/relational_graph_decidable_IG_operations.v
@@ -1,0 +1,202 @@
+
+
+Require Import String.
+
+Require Import List.
+Import ListNotations.
+
+
+Require Import Bool.
+Require Import Coq.Sorting.Permutation.
+
+
+Require Import MyProject.project.relational_graph_decidable.
+Require Import MyProject.project.util.util.
+Require Import MyProject.project.util.NatMap.
+
+Require Import Coq.Arith.Arith.
+
+Open Scope nat_scope.
+
+
+
+
+
+(* Defines the IG functions in terms of an RG (notice that it has generic edge or node label types) *)
+
+
+  (* {-# MINIMAL empty, isEmpty, match, mkGraph, labNodes #-} *)
+
+(* These are the interfacing types of an IG _copied_ from the paper *)
+(* type Adj b = [(b, Node)] *)
+Definition Adj (B : Type) := list (B * Node).
+
+(* type Context a b  = (Adj b,Node,a,Adj b) *)
+Definition Context (A B : Type) : Type := (Adj B * Node * A * Adj B)%type.
+
+(* type Decomp g a b = (MContext a b,g a b) *)
+Definition Decomp (A B : Type) := (option (Context A B) * RG_dec A B)%type. 
+
+(* type LEdge b = (Node,Node,b) *)
+Definition LEdge (B : Type) :=  (Node * Node * B)%type. 
+
+(* type LNode a = (Node,a) *)
+Definition LNode (A : Type) :=  (Node * A)%type.
+
+
+
+(* Defining equivalences for the sake of proving stuff *)
+
+Definition Adj_equiv {B : Type} (adj1 adj2 : Adj B) : Prop :=
+  Permutation adj1 adj2
+. 
+
+Notation "adj1 A== adj2" := (Adj_equiv adj1 adj2) (at level 100, right associativity).
+
+
+Definition Context_equiv {A B : Type} (c1 c2 : Context A B) : Prop :=
+  match c1, c2 with | (fromsC1, nC1, lC1, tosC1), (fromsC2, nC2, lC2, tosC2) =>
+      Adj_equiv fromsC1 fromsC2 /\ nC1 = nC2 /\ lC1 = lC2 /\ Adj_equiv tosC1 tosC2
+  end
+.
+
+Notation "c1 C== c2" := (Context_equiv c1 c2) (at level 79, right associativity).
+
+Definition Decomp_equiv {A B : Type} (d1 d2 : Decomp A B) : Prop :=
+  match d1, d2 with
+    | (Some (context1), rg1), (Some (context2), rg2) =>
+      context1 C== context2 /\ (rg1 === rg2)
+    | (None, rg1), (None, rg2) =>
+      rg1 === rg2
+    | _, _ => False
+  end
+.
+
+Notation "c1 D== c2" := (Decomp_equiv c1 c2) (at level 79, right associativity).
+
+
+(* Start defining functionality: *)
+Print RG_dec_empty.
+(* Definition RG_empty {A B} : RG A B :=
+    RG_empty. *)
+
+Print RG_dec_isEmpty.
+(* Definition RG_isEmpty {A B: Type} (rg : RG A B) : Prop :=
+  RG_isEmpty rg. *)
+
+
+
+(* Helper for match *)
+(* Removes a node from the nodeset and any edges *)
+Definition _eliminate {A B : Type} (node : Node) (rg : RG_dec A B) : RG_dec A B.
+Proof.
+  refine {|
+      RG_dec_nodes := NatMap.remove node rg.(RG_dec_nodes); 
+      RG_dec_edges := filter_map (fun '((from, to) : (nat*nat)) labels => negb ((from =? node) || (to =? node))) rg.(RG_dec_edges); 
+      RG_dec_valid := _
+  |}.
+Admitted.
+
+Check fold_right.
+(* (B -> A -> A) -> A -> list B -> A *)
+
+(* Checks if the node is in the RG_dec (the Prop return) and returns two sets of alls incoming neighbors and outgoing neighbors *)
+Definition _getFromsAndTos {A B : Type} (node : Node) (rg : RG_dec A B) : option (Context A B) :=
+  match NatMap.find node rg.(RG_dec_nodes) with
+    | Some _ => match NatMap.find node rg.(RG_dec_nodes) with
+                 | Some label => Some (
+                  fold_right (fun '((n, l) : Node * A) acc => 
+                        let edges := PairNatMap.find (n, node) rg.(RG_dec_edges) in
+                        match edges with
+                          | Some edges => (map (fun '(b : B) => (b, n)) edges) ++ acc
+                          | None => acc
+                        end
+                 ) [] (NatMap.elements rg.(RG_dec_nodes))
+                 
+                 ,
+                                   node,
+                                   label,
+                                   fold_right (fun '((n, l) : Node * A) acc => 
+                        let edges := PairNatMap.find (node, n) rg.(RG_dec_edges) in
+                        match edges with
+                          | Some edges => (map (fun '(b : B) => (b, n)) edges) ++ acc
+                          | None => acc
+                        end
+                 ) [] (NatMap.elements rg.(RG_dec_nodes))
+                 )
+                                   
+                 | None => None
+               end
+    | None => None
+  end
+.
+
+
+(* The code for match is basically as complicated as the code for match on a "real" rg.... *)
+Definition RG_dec_match {A B : Type} (node : Node) (rg : RG_dec A B) : Decomp A B :=
+  (_getFromsAndTos node rg, _eliminate node rg)
+.
+
+
+(* Definition _add {A B : Type} (context : RG_dec_Context A B) (rg : RG_dec A B) : RG_dec A B.
+Proof.
+  destruct context as [[froms node] tos].
+  Print RG_dec_Adj.
+  refine {|
+      RG_dec_nodes := fun (n : A) =>  (exists l, froms l n) \/
+                                  (exists l, tos l n) \/
+                                  cEnsembleAdd node rg.(RG_dec_nodes) n;
+      RG_dec_edges := fun (n1 n2 : A) (l : B) =>  (froms l n1 /\ n2 = node) \/
+                                              (n1 = node /\ tos l n2) \/ 
+                                              rg.(RG_dec_edges) n1 n2 l;
+      RG_dec_valid := _
+  |}.
+  RG_dec_valid_prover_with rg.
+Defined. *)
+
+
+Definition _insNode {A B : Type} (node : LNode A) (rg : RG_dec A B) : RG_dec A B.
+Proof.
+  destruct node as [n l].
+    refine {|
+      RG_dec_nodes := NatMap.add n l rg.(RG_dec_nodes);
+      RG_dec_edges := rg.(RG_dec_edges);
+      RG_dec_valid := _
+  |}.
+Admitted.
+
+
+Definition _insNodes {A B : Type} (nodes : list (LNode A)) (rg : RG_dec A B) : RG_dec A B :=
+  fold_right _insNode rg nodes.
+
+
+Definition update_with_default {A : Type} (f : A -> A) (d : A) (k : PairNatMap.key) (m : PairNatMap.t A) : PairNatMap.t A :=
+  let v := match PairNatMap.find k m with
+           | Some x => x
+           | None => d
+           end in
+  PairNatMap.add k (f v) m.
+
+(* If one of the nodes of the edge does not exist, nothing happens *)
+Definition _insEdge {A B : Type} (edge : LEdge B) (rg : RG_dec A B) : RG_dec A B. 
+Proof.
+  destruct edge as [[from to] l].
+    refine {|
+      RG_dec_nodes := rg.(RG_dec_nodes);
+      RG_dec_edges := update_with_default (fun labels => l::labels) [l] (from, to) rg.(RG_dec_edges);
+      RG_dec_valid := _
+  |}.
+Admitted.
+
+
+Definition _insEdges {A B : Type} (edges : list (LEdge B)) (rg : RG_dec A B) : RG_dec A B :=
+  fold_right _insEdge rg edges.
+
+Definition RG_dec_mkGraph {A B : Type} (nodes : list (LNode A)) (edges : list (LEdge B)) : RG_dec A B :=
+  _insEdges edges (_insNodes nodes RG_dec_empty).
+ 
+
+Definition RG_dec_labNodes {A B : Type} (rg : RG_dec A B) : list (LNode A) :=
+  NatMap.elements rg.(RG_dec_nodes).
+
+
