project/util/NatMap.v
@@ -1,0 +1,39 @@
+Require Import FMaps.
+
+
+Definition Node := Nat_as_OT.t.
+
+Module NatMap := FMapList.Make(Nat_as_OT).
+
+Module WF := WFacts_fun Nat_as_OT NatMap. (* Library of useful lemmas about maps *)
+Module WP := WProperties_fun Nat_as_OT NatMap. (* More useful stuff about maps *)
+Print Module WF.
+Print Module WP.
+Check Nat_as_OT.lt. (*   : positive -> positive -> Prop *)
+
+
+
+Module PairNat_as_OT := PairOrderedType(Nat_as_OT)(Nat_as_OT).
+Definition NodePair := PairNat_as_OT.t.
+
+Module PairNatMap := FMapList.Make(PairNat_as_OT).
+
+Module PWF := WFacts_fun PairNat_as_OT PairNatMap. (* Library of useful lemmas about maps *)
+Module PWP := WProperties_fun PairNat_as_OT PairNatMap. (* More useful stuff about maps *)
+
+
+
+Definition filter_map {A : Type} (pred : PairNatMap.key -> A -> bool) (m : PairNatMap.t A) : PairNatMap.t A :=
+  PairNatMap.fold (fun k v acc =>
+            if pred k v then PairNatMap.add k v acc else acc)
+         m
+         (PairNatMap.empty A)
+.
+
+
+(* Definition myPairNatMap : PairNatMap.t nat := PairNatMap.empty nat.
+Definition myPairNatMap' := PairNatMap.add (1, 2) 3 myPairNatMap.
+Compute PairNatMap.find (1, 2) myPairNatMap'.
+Definition isIn (keys : nat * nat) (map : PairNatMap.t nat) := PairNatMap.In keys map.
+Compute PairNatMap.In (1, 2) myPairNatMap'. *)
+
