project/util/NatSet.v
@@ -1,6 +1,9 @@
 Require Import FSets.
 
+
+(* TODO: migrate to Msets *)
 Definition Node := Nat_as_OT.t.
 
 Module NatSet := FSetList.Make(Nat_as_OT).
 Module NatSetProperties := EqProperties(NatSet).
+
